theories/Inert.v
@@ -17,6 +17,12 @@ Definition i_ub i1 i2 i3 :=
 Arguments i_ub i1 i2 i3/.
 Hint Unfold i_ub : i1 i2 i3.
 
+Theorem i_ub_inert : forall i1 i2, i_ub i1 i2 Inert -> i1 = Inert /\ i2 = Inert.
+Proof.
+best.
+Qed.
+
+
 (* if i is required to be inert, then p must hold.*)
 Definition inert_guard (p : Prop) (i : inertness) : Prop :=
   i = Inert -> p.
