theories/Nullable.v
@@ -1,7 +1,9 @@
+Require Import Coq.Program.Equality.
 From LambdaST Require Import
   Context
   Prefix
   Types.
+From Hammer Require Import Tactics.
 
 Inductive Nullable : type -> Prop :=
   | NullableTyEps : Nullable TyEps
@@ -20,3 +22,13 @@ Inductive NullableCtx : context -> Prop :=
       NullableCtx (CtxComma G G')
   .
 Hint Constructors NullableCtx : core.
+
+Theorem hmm'' : forall p s,
+  EmptyPrefix p ->
+  MaximalPrefix p ->
+  PrefixTyped p s ->
+  Nullable s.
+Proof.
+  intros p s He Hm Ht.
+  dependent induction Ht; sauto lq: on.
+Qed.
